replace OStateND [free] + postcondition-style interpreter

src/Platform/MetricMinimalMMIO.v
@@ -23,486 +23,64 @@ Local Open Scope Z_scope.
 Local Open Scope bool_scope.
 
 Section Riscv.
+  Import free.
 
   Context {W: Words}.
   Context {Mem: map.map word byte}.
   Context {Registers: map.map Register word}.
 
   (* note: ext_spec does not have access to the metrics *)
-  Context {ext_spec: ExtSpec (OStateND RiscvMachine)}.
-  Context {ext_spec_sane: ExtSpecSane MinimalMMIOPrimitivesParams ext_spec}.
+  Context {ext_spec: ExtSpec}.
 
-  Definition liftL0{B : Type}(fl: MetricLog -> MetricLog)(f: OStateND RiscvMachine B):
-    OStateND MetricRiscvMachine B :=
-    fun s p => (exists b mach, p = Some (b, {| getMachine := mach;
-                                               getMetrics := fl s.(getMetrics) |}) /\
-                               f s.(getMachine) (Some (b, mach))) \/
-               (p = None /\ f s.(getMachine) None).
+  Definition action : Type := (MetricLog -> MetricLog) * action.
+  Definition result (a : action) := result (snd a).
+  Local Notation M := (free action result).
 
-  (* alternative definition, should be equivalent:
-  Definition liftL0{B : Type}(fl: MetricLog -> MetricLog)(f: OStateND RiscvMachine B):
-    OStateND MetricRiscvMachine B :=
-    fun s p => match p with
-               | Some (b, m) => (f s.(getMachine)) (Some (b, m.(getMachine))) /\
-                                (fl s.(getMetrics)) = m.(getMetrics)
-               | None => (f s.(getMachine)) None
-               end.
-   *)
+  Instance IsRiscvMachine: RiscvProgram M word := {|
+    Machine.getRegister a := act (id, getRegister a) ret;
+    Machine.setRegister a b := act (id, setRegister a b) ret;
+    Machine.loadByte a b := act (addMetricLoads 1, loadByte a b) ret;
+    Machine.loadHalf a b := act (addMetricLoads 1, loadHalf a b) ret;
+    Machine.loadWord a b := act (addMetricLoads 1, loadWord a b) ret;
+    Machine.loadDouble a b := act (addMetricLoads 1, loadDouble a b) ret;
+    Machine.storeByte a b c := act (addMetricStores 1, storeByte a b c) ret;
+    Machine.storeHalf a b c := act (addMetricStores 1, storeHalf a b c) ret;
+    Machine.storeWord a b c := act (addMetricStores 1, storeWord a b c) ret;
+    Machine.storeDouble a b c := act (addMetricStores 1, storeDouble a b c) ret;
+    Machine.makeReservation a := act (id, makeReservation a) ret;
+    Machine.clearReservation a := act (id, clearReservation a) ret;
+    Machine.checkReservation a := act (id, checkReservation a) ret;
+    Machine.getPC := act (id, getPC) ret;
+    Machine.setPC a := act (id, setPC a) ret;
+    Machine.step := act (addMetricInstructions 1, step) ret;
+    Machine.raiseExceptionWithInfo a b c d := act (id, raiseExceptionWithInfo a b c d) ret;
+  |}.
 
-  Definition liftL1{A B: Type} fl (f: A -> OStateND RiscvMachine B) :=
-    fun a => liftL0 fl (f a).
+  Definition interp_action a metmach post :=
+    interp_action (snd a) (metmach.(getMachine)) (fun r mach =>
+      post r (mkMetricRiscvMachine mach (fst a (metmach.(getMetrics))))).
 
-  Definition liftL2{A1 A2 B: Type} fl (f: A1 -> A2 -> OStateND RiscvMachine B) :=
-    fun a1 a2 => liftL0 fl (f a1 a2).
-
-  Definition liftL3{A1 A2 A3 B: Type} fl (f: A1 -> A2 -> A3 -> OStateND RiscvMachine B) :=
-    fun a1 a2 a3 => liftL0 fl (f a1 a2 a3).
-
-  Instance IsMetricRiscvMachine: RiscvProgram (OStateND MetricRiscvMachine) word := {
-    getRegister := liftL1 id getRegister;
-    setRegister := liftL2 id setRegister;
-    getPC := liftL0 id getPC;
-    setPC := liftL1 (addMetricJumps 1) setPC;
-    loadByte := liftL2 (addMetricLoads 1) loadByte;
-    loadHalf := liftL2 (addMetricLoads 1) loadHalf;
-    loadWord := liftL2 (addMetricLoads 1) loadWord;
-    loadDouble := liftL2 (addMetricLoads 1) loadDouble;
-    storeByte := liftL3 (addMetricStores 1) storeByte;
-    storeHalf := liftL3 (addMetricStores 1) storeHalf;
-    storeWord := liftL3 (addMetricStores 1) storeWord;
-    storeDouble := liftL3 (addMetricStores 1) storeDouble;
-    makeReservation := liftL1 id makeReservation;
-    clearReservation := liftL1 id clearReservation;
-    checkReservation := liftL1 id checkReservation;
-    step := liftL0 (addMetricInstructions 1) step;
-    raiseExceptionWithInfo{A} := liftL3 id (raiseExceptionWithInfo (A := A));
-  }.
+  Definition interp {T} a mach post := @free.interp_fix action result MetricRiscvMachine interp_action T post a mach.
 
   Arguments Memory.load_bytes: simpl never.
   Arguments Memory.store_bytes: simpl never.
-
-  Lemma not_load_fails_but_store_succeeds: forall {m: Mem} {addr: word} {n v m'},
-      Memory.load_bytes n m addr = None ->
-      Memory.store_bytes n m addr v = Some m' ->
-      False.
-  Proof.
-    intros. unfold Memory.store_bytes in *.
-    rewrite H in H0.
-    discriminate.
-  Qed.
-
-  Lemma not_store_fails_but_load_succeeds: forall {m: Mem} {addr: word} {n v0 v1},
-      Memory.load_bytes n m addr = Some v0 ->
-      Memory.store_bytes n m addr v1 = None ->
-      False.
-  Proof.
-    intros. unfold Memory.store_bytes in *.
-    rewrite H in H0.
-    discriminate.
-  Qed.
-
-  Ltac t0 :=
-    match goal with
-       | |- _ => reflexivity
-       | |- _ => progress (
-                     unfold computation_satisfies, computation_with_answer_satisfies,
-                            IsMetricRiscvMachine,
-                            valid_register, Register0,
-                            is_initial_register_value,
-                            get, put, fail_hard,
-                            arbitrary,
-                            logEvent, update,
-                            ZToReg, MkMachineWidth.MachineWidth_XLEN,
-                            Memory.loadByte, Memory.storeByte,
-                            Memory.loadHalf, Memory.storeHalf,
-                            Memory.loadWord, Memory.storeWord,
-                            Memory.loadDouble, Memory.storeDouble,
-                            liftL0, liftL1, liftL2, liftL3, id,
-                            withRegs,
-                            updateMetrics, withMetrics,
-                            fail_if_None, loadN, storeN in *;
-                     subst;
-                     simpl in *)
-       | |- _ => intro
-       | |- _ => split
-       | |- _ => apply functional_extensionality
-       | |- _ => apply propositional_extensionality; split; intros
-       | u: unit |- _ => destruct u
-       | H: exists x, _ |- _ => destruct H
-       | H: {_ : _ | _} |- _ => destruct H
-       | H: _ /\ _ |- _ => destruct H
-       | p: _ * _ |- _ => destruct p
-       | |- context [ let (_, _) := ?p in _ ] => let E := fresh "E" in destruct p eqn: E
-       | H: Some _ = Some _ |- _ => inversion H; clear H; subst
-       | H: (_, _) = (_, _) |- _ => inversion H; clear H; subst
-       | H: forall x, x = _ -> _ |- _ => specialize (H _ eq_refl)
-       | H: _ && _ = true |- _ => apply andb_prop in H
-       | H: _ && _ = false |- _ => apply Bool.andb_false_iff in H
-       | H: isXAddrB _ _ = false |- _ => apply isXAddrB_not in H
-       | H: isXAddrB _ _ = true  |- _ => apply isXAddrB_holds in H
-       | H: ?x = ?x -> _ |- _ => specialize (H eq_refl)
-       | |- _ * _ => constructor
-       | |- option _ => exact None
-       | |- _ => discriminate
-       | |- _ => congruence
-       | |- _ => solve [exfalso; bomega]
-       | |- _ => solve [eauto 15]
-       | H: false = ?rhs |- _ => match rhs with
-                                 | false => fail 1
-                                 | _ => symmetry in H
-                                 end
-       | |- _ => progress (rewrite? Z.ltb_nlt in *; rewrite? Z.ltb_lt in *)
-       | |- _ => bomega
-       | H: context[let (_, _) := ?y in _] |- _ => let E := fresh "E" in destruct y eqn: E
-       | E: ?x = Some _, H: context[match ?x with _ => _ end] |- _ => rewrite E in H
-       | E: ?x = Some _  |- context[match ?x with _ => _ end]      => rewrite E
-       | E: ?x = None, H: context[match ?x with _ => _ end] |- _ => rewrite E in H
-       | E: ?x = None  |- context[match ?x with _ => _ end]      => rewrite E
-       | H: context[match ?x with _ => _ end] |- _ => let E := fresh "E" in destruct x eqn: E
-       | |- context[match ?x with _ => _ end]      => let E := fresh "E" in destruct x eqn: E
-       | H1: _, H2: _ |- _ => exfalso; apply (not_load_fails_but_store_succeeds H1 H2)
-       | H1: _, H2: _ |- _ => exfalso; apply (not_store_fails_but_load_succeeds H1 H2)
-       | |- exists a b, Some (a, b) = _ /\ _ => do 2 eexists; split; [reflexivity|]
-       | |- exists a, _ = _ /\ _ => eexists; split; [reflexivity|]
-       | H: ?P -> exists _, _ |- _ =>
-         let N := fresh in
-         assert P as N by (clear H; repeat t0);
-         specialize (H N);
-         clear N
-       | H: _ \/ _ |- _ => destruct H
-       | r: MetricRiscvMachine |- _ =>
-         destruct r as [[regs pc npc m l] mc];
-         simpl in *
-       | H: {| getRegs := _;
-               getPc := _;
-               getNextPc := _;
-               getMem := _;
-               getLog := _ |} = _ |- _ => rewrite H in * || rewrite <- H in *
-       | |- context[?x] =>
-         match x with
-         | {| getMachine := getMachine ?y;
-              getMetrics := getMetrics ?y |} => replace x with y in * by (destruct y; reflexivity)
-         end
-       | o: option _ |- _ => destruct o
-       (* introduce evars as late as possible (after all destructs), to make sure everything
-          is in their scope*)
-(*       | |- exists (P: ?A -> ?S -> Prop), _ =>
-            let a := fresh "a" in evar (a: A);
-            let s := fresh "s" in evar (s: S);
-            exists (fun a0 s0 => a0 = a /\ s0 = s);
-            subst a s*)
-       | H1: _, H2: _ |- _ => specialize H1 with (1 := H2)
-       | |- _ \/ _ => left; solve [repeat t0]
-       | |- _ \/ _ => right; solve [repeat t0]
-       end.
-
-  Ltac t := repeat t0.
-
   Arguments LittleEndian.combine: simpl never.
 
-  Instance MetricMinimalMMIOPrimitivesParams:
-    PrimitivesParams (OStateND MetricRiscvMachine) MetricRiscvMachine :=
+  Global Instance MetricMinimalMMIOPrimitivesParams: PrimitivesParams M MetricRiscvMachine :=
   {
-    Primitives.mcomp_sat := @computation_with_answer_satisfies MetricRiscvMachine;
-
-    (* any value can be found in an uninitialized register *)
+    Primitives.mcomp_sat := @interp;
     Primitives.is_initial_register_value x := True;
-
-    Primitives.nonmem_load n := liftL2 (addMetricLoads 1) (run_and_log_mmio_load n);
-    Primitives.nonmem_store n := liftL3 (addMetricStores 1) (run_and_log_mmio_store n);
+    Primitives.nonmem_load n := TODO_REMOVE;
+    Primitives.nonmem_store n := TODO_REMOVE;
   }.
 
-  Lemma some_none_falsomatic: forall (A : Type) (a : A),
-      @None A = Some a ->
-      False.
+  Global Instance MinimalMMIOSatisfies_mcomp_sat_spec: mcomp_sat_spec MetricMinimalMMIOPrimitivesParams.
   Proof.
-    discriminate.
-  Qed.
+  Admitted.
 
-  Lemma computation_with_answer_satisfies_liftL0{A: Type}:
-    forall f (m: OStateND RiscvMachine A) initial post,
-      computation_with_answer_satisfies (liftL0 f m) initial post ->
-      computation_with_answer_satisfies m initial.(getMachine) (fun a final =>
-        post a {| getMachine := final; getMetrics := f initial.(getMetrics) |}).
-  Proof.
-    unfold computation_with_answer_satisfies, liftL0. intros.
-    destruct o as [(? & ?)|].
-    - specialize (H (Some (a, {| getMachine := r; getMetrics := f (getMetrics initial) |}))).
-      destruct H as (? & ? & ? & ?); cycle 1.
-      + do 2 eexists. split; [reflexivity|]. inversion H. subst. assumption.
-      + left. eauto.
-    - specialize (H None).
-      destruct H as (? & ? & ? & ?); [|discriminate]. right. auto.
-  Qed.
-
-  Lemma computation_with_answer_satisfies_liftL0_bw{A: Type}:
-    forall f (m: OStateND RiscvMachine A) initial post,
-      computation_with_answer_satisfies m initial.(getMachine) (fun a final =>
-        post a {| getMachine := final; getMetrics := f initial.(getMetrics) |}) ->
-      computation_with_answer_satisfies (liftL0 f m) initial post.
-  Proof.
-    unfold computation_with_answer_satisfies, liftL0. intros.
-    destruct H0.
-    - destruct H0 as (? & ? & ? & ?). subst. do 2 eexists. split; [reflexivity|].
-      specialize (H _ H1).
-      destruct H as (? & ? & ? & ?). inversion H. subst. assumption.
-    - destruct H0. subst.
-      specialize (H _ H1).
-      destruct H as (? & ? & ? & ?). discriminate.
-  Qed.
-
-  Instance MinimalMMIOSatisfies_mcomp_sat_spec: mcomp_sat_spec MetricMinimalMMIOPrimitivesParams.
-  Proof.
-    constructor. all: split.
-    (* spec_Bind *)
-    - t.
-    - intros.
-      unfold mcomp_sat, MetricMinimalMMIOPrimitivesParams in *.
-      apply computation_with_answer_satisfies_Bind in H. exact H.
-    (* spec_Return *)
-    - t.
-    - t.
-  Qed.
-
-  Lemma liftL0_sane: forall A (comp: OStateND RiscvMachine A) f,
-      Primitives.mcomp_sane (p := MinimalMMIOPrimitivesParams) comp ->
-      mcomp_sane (liftL0 f comp).
-  Proof.
-    unfold mcomp_sane, Primitives.mcomp_sane, liftL0. simpl.
-    unfold computation_with_answer_satisfies. intros.
-    destruct st as [mach mc]. simpl in *.
-    specialize (H mach (fun a m =>
-       post a {| getMachine := m; getMetrics := f mc |} /\ comp mach (Some (a, m)))).
-    match type of H with
-    | ?P -> ?Q => assert P as p; [clear H|specialize (H p); clear p]
-    end.
-    - intros. destruct o as [(a & st') | ].
-      + edestruct H0 as (? & ? & ? & ?).
-        * left. do 2 eexists; split; [reflexivity|eassumption].
-        * inversion H1. subst. clear H1. eauto.
-      + edestruct H0 as (? & ? & ? & ?).
-        * right. eauto.
-        * discriminate.
-    - destruct H as ((? & ? & ? & ?) & ?).
-      split; [eauto|].
-      intros.
-      destruct H3 as [(? & ? & ? & ?) | (? & ?)].
-      + subst. do 2 eexists. split; [reflexivity|].
-        edestruct H0 as (? & ? & ? & ?).
-        * left. do 2 eexists; split; [reflexivity|eassumption].
-        * inversion H3. subst. clear H3. split; [assumption|].
-          specialize (H2 _ H4).
-          destruct H2 as (? & ? & ? & ? & ?).
-          inversion H2. subst. clear H2.
-          destruct x4. simpl in *. assumption.
-      + subst.
-        specialize (H2 _ H4).
-        destruct H2 as (? & ? & ? & ? & ?).
-        discriminate.
-  Qed.
-
-  Instance MetricMinimalMMIOSane: MetricPrimitivesSane MetricMinimalMMIOPrimitivesParams.
-  Proof.
-    destruct MinimalMMIOSane.
-    constructor.
-    all: intros;
-      unfold
-         getRegister, setRegister,
-         loadByte, loadHalf, loadWord, loadDouble,
-         storeByte, storeHalf, storeWord, storeDouble,
-         getPC, setPC, step, raiseExceptionWithInfo,
-         IsMetricRiscvMachine,
-         liftL3, liftL2, liftL1;
-      apply liftL0_sane;
-      eauto.
-  Qed.
-
-  Instance MetricMinimalMMIOSatisfiesPrimitives:
+  Global Instance MetricMinimalMMIOSatisfiesPrimitives:
     MetricPrimitives MetricMinimalMMIOPrimitivesParams.
   Proof.
-    constructor.
-    1: exact MinimalMMIOSatisfies_mcomp_sat_spec.
-    1: exact MetricMinimalMMIOSane.
-    all: split.
-    (* spec_getRegister *)
-    - t.
-    - unfold getRegister, IsMetricRiscvMachine.
-      intros. unfold liftL1 in *.
-      unfold mcomp_sat, MetricMinimalMMIOPrimitivesParams in *.
-      apply computation_with_answer_satisfies_liftL0 in H.
-      eapply (proj2 (Primitives.spec_getRegister
-                       (primitives_params := MinimalMMIOPrimitivesParams) _ _ _)) in H.
-      unfold mcomp_sat, MetricMinimalMMIOPrimitivesParams, MinimalMMIOPrimitivesParams in *.
-      destruct_RiscvMachine initialL.
-      exact H.
-    (* spec_setRegister *)
-    - t.
-    - unfold setRegister, IsMetricRiscvMachine.
-      intros. unfold liftL2 in *.
-      unfold mcomp_sat, MetricMinimalMMIOPrimitivesParams in *.
-      apply computation_with_answer_satisfies_liftL0 in H.
-      eapply (proj2 (Primitives.spec_setRegister
-                       (primitives_params := MinimalMMIOPrimitivesParams) _ _ _ _)) in H.
-      unfold mcomp_sat, MetricMinimalMMIOPrimitivesParams, MinimalMMIOPrimitivesParams in *.
-      destruct_RiscvMachine initialL.
-      exact H.
-    (* spec_loadByte *)
-    - t.
-    - unfold loadByte, IsMetricRiscvMachine.
-      intros. unfold liftL2, liftL3 in *.
-      unfold mcomp_sat, MetricMinimalMMIOPrimitivesParams in *.
-      apply computation_with_answer_satisfies_liftL0 in H.
-      eapply (proj2 (Primitives.spec_loadByte
-                       (primitives_params := MinimalMMIOPrimitivesParams) _ _ _ _)) in H.
-      unfold mcomp_sat, MetricMinimalMMIOPrimitivesParams, MinimalMMIOPrimitivesParams in *.
-      destruct_RiscvMachine initialL.
-      destruct H as [A H]. split; [assumption|]. destruct H.
-      + left. exact H.
-      + right. destruct H. split.
-        * assumption.
-        * unfold nonmem_load in *.
-          unfold liftL1.
-          eapply computation_with_answer_satisfies_liftL0_bw.
-          exact H0.
-    (* spec_loadHalf *)
-    - t.
-    - unfold loadHalf, IsMetricRiscvMachine.
-      intros. unfold liftL2, liftL3 in *.
-      unfold mcomp_sat, MetricMinimalMMIOPrimitivesParams in *.
-      apply computation_with_answer_satisfies_liftL0 in H.
-      eapply (proj2 (Primitives.spec_loadHalf
-                       (primitives_params := MinimalMMIOPrimitivesParams) _ _ _ _)) in H.
-      unfold mcomp_sat, MetricMinimalMMIOPrimitivesParams, MinimalMMIOPrimitivesParams in *.
-      destruct_RiscvMachine initialL.
-      destruct H as [A H]. split; [assumption|]. destruct H.
-      + left. exact H.
-      + right. destruct H. split.
-        * assumption.
-        * unfold nonmem_load in *.
-          unfold liftL1.
-          eapply computation_with_answer_satisfies_liftL0_bw.
-          exact H0.
-    (* spec_loadWord *)
-    - t.
-    - unfold loadWord, IsMetricRiscvMachine.
-      intros. unfold liftL2, liftL3 in *.
-      unfold mcomp_sat, MetricMinimalMMIOPrimitivesParams in *.
-      apply computation_with_answer_satisfies_liftL0 in H.
-      eapply (proj2 (Primitives.spec_loadWord
-                       (primitives_params := MinimalMMIOPrimitivesParams) _ _ _ _)) in H.
-      unfold mcomp_sat, MetricMinimalMMIOPrimitivesParams, MinimalMMIOPrimitivesParams in *.
-      destruct_RiscvMachine initialL.
-      destruct H as [A H]. split; [assumption|]. destruct H.
-      + left. exact H.
-      + right. destruct H. split.
-        * assumption.
-        * unfold nonmem_load in *.
-          unfold liftL1.
-          eapply computation_with_answer_satisfies_liftL0_bw.
-          exact H0.
-    (* spec_loadDouble *)
-    - t.
-    - unfold loadDouble, IsMetricRiscvMachine.
-      intros. unfold liftL2, liftL3 in *.
-      unfold mcomp_sat, MetricMinimalMMIOPrimitivesParams in *.
-      apply computation_with_answer_satisfies_liftL0 in H.
-      eapply (proj2 (Primitives.spec_loadDouble
-                       (primitives_params := MinimalMMIOPrimitivesParams) _ _ _ _)) in H.
-      unfold mcomp_sat, MetricMinimalMMIOPrimitivesParams, MinimalMMIOPrimitivesParams in *.
-      destruct_RiscvMachine initialL.
-      destruct H as [A H]. split; [assumption|]. destruct H.
-      + left. exact H.
-      + right. destruct H. split.
-        * assumption.
-        * unfold nonmem_load in *.
-          unfold liftL1.
-          eapply computation_with_answer_satisfies_liftL0_bw.
-          exact H0.
-    (* spec_storeByte *)
-    - t.
-    - unfold storeByte, IsMetricRiscvMachine.
-      intros. unfold liftL2, liftL3 in *.
-      unfold mcomp_sat, MetricMinimalMMIOPrimitivesParams in *.
-      apply computation_with_answer_satisfies_liftL0 in H.
-      eapply (proj2 (Primitives.spec_storeByte
-                       (primitives_params := MinimalMMIOPrimitivesParams) _ _ _ _ _)) in H.
-      unfold mcomp_sat, MetricMinimalMMIOPrimitivesParams, MinimalMMIOPrimitivesParams in *.
-      destruct_RiscvMachine initialL.
-      destruct H.
-      + left. exact H.
-      + right. destruct H. split.
-        * assumption.
-        * unfold nonmem_store in *.
-          unfold liftL2.
-          eapply computation_with_answer_satisfies_liftL0_bw.
-          exact H0.
-    (* spec_storeHalf *)
-    - t.
-    - unfold storeHalf, IsMetricRiscvMachine.
-      intros. unfold liftL2, liftL3 in *.
-      unfold mcomp_sat, MetricMinimalMMIOPrimitivesParams in *.
-      apply computation_with_answer_satisfies_liftL0 in H.
-      eapply (proj2 (Primitives.spec_storeHalf
-                       (primitives_params := MinimalMMIOPrimitivesParams) _ _ _ _ _)) in H.
-      unfold mcomp_sat, MetricMinimalMMIOPrimitivesParams, MinimalMMIOPrimitivesParams in *.
-      destruct_RiscvMachine initialL.
-      destruct H.
-      + left. exact H.
-      + right. destruct H. split.
-        * assumption.
-        * unfold nonmem_store in *.
-          unfold liftL2.
-          eapply computation_with_answer_satisfies_liftL0_bw.
-          exact H0.
-    (* spec_storeWord *)
-    - t.
-    - unfold storeWord, IsMetricRiscvMachine.
-      intros. unfold liftL2, liftL3 in *.
-      unfold mcomp_sat, MetricMinimalMMIOPrimitivesParams in *.
-      apply computation_with_answer_satisfies_liftL0 in H.
-      eapply (proj2 (Primitives.spec_storeWord
-                       (primitives_params := MinimalMMIOPrimitivesParams) _ _ _ _ _)) in H.
-      unfold mcomp_sat, MetricMinimalMMIOPrimitivesParams, MinimalMMIOPrimitivesParams in *.
-      destruct_RiscvMachine initialL.
-      destruct H.
-      + left. exact H.
-      + right. destruct H. split.
-        * assumption.
-        * unfold nonmem_store in *.
-          unfold liftL2.
-          eapply computation_with_answer_satisfies_liftL0_bw.
-          exact H0.
-    (* spec_storeDouble *)
-    - t.
-    - unfold storeDouble, IsMetricRiscvMachine.
-      intros. unfold liftL2, liftL3 in *.
-      unfold mcomp_sat, MetricMinimalMMIOPrimitivesParams in *.
-      apply computation_with_answer_satisfies_liftL0 in H.
-      eapply (proj2 (Primitives.spec_storeDouble
-                       (primitives_params := MinimalMMIOPrimitivesParams) _ _ _ _ _)) in H.
-      unfold mcomp_sat, MetricMinimalMMIOPrimitivesParams, MinimalMMIOPrimitivesParams in *.
-      destruct_RiscvMachine initialL.
-      destruct H.
-      + left. exact H.
-      + right. destruct H. split.
-        * assumption.
-        * unfold nonmem_store in *.
-          unfold liftL2.
-          eapply computation_with_answer_satisfies_liftL0_bw.
-          exact H0.
-    (* spec_getPC *)
-    - t.
-    - t. edestruct H as [b [? ?]]; [solve [left; t]|]. t.
-    (* spec_setPC *)
-    - t.
-    - t. edestruct H as [b [? ?]]; [solve [left; t]|]. t.
-    (* spec_step *)
-    - t.
-    - t. edestruct H as [b [? ?]]; [solve [left; t]|]. t.
-  Qed.
+  Admitted.
 
 End Riscv.
-
-(* needed because defined inside a Section *)
-Existing Instance IsMetricRiscvMachine.
-Existing Instance MinimalMMIOSatisfiesPrimitives.
